#Examples
#####Example1 [Deprecated]
$$
{\begin{cases}
my''+ky=\delta(t),\\
y_0=y(0)=y(0_{\_})
\end{cases}}
\Rightarrow
{\begin{cases}
my''+ky=0,\\
y_0=y(0)=y(0_{+}), \text{where }y(0_{+})-y(0_{\_})=\frac{1}{m}
\end{cases}}
$$
#####Example2
?source
$$
\begin{cases}
y''+2y'-15y=6\delta(t-9),\\
y_0=y(0)=-5\\
y_1=y'(0)=7
\end{cases}
$$
Solution:
$$
f(t)=\frac{1}{8}e^{3t}-\frac{1}{8}e^{-5t},\text{ }g(t)=\frac{9}{4}e^{3t}+\frac{11}{4}e^{-5t}\\
y(t)=6H(t,9)f(t-9)-g(t)
$$
#####Example3 [Finan, p.57]
$$
\begin{cases}
2y''+4y'+10y=\delta(t),\\
y_0=y(0)=0\\
y_1=y'(0)=0
\end{cases}
$$
Solution:
$$
x(t)=\frac{1}{4}e^{-2t}sin(2t)
$$
#####Example4
?source
$$
\begin{cases}
y''+3y'+2y=2\delta(t-3),\\
y_0=y(0)=0\\
y_1=y'(0)=1
\end{cases}
$$
Solution:
$$
y(t)=\frac{1}{2}e^{t}sin(2t)+H(t,3)e^{t-3}sin(2t-6)
$$
#####Example5.1 [Zill, p.293]
$$
\begin{cases}
y''+y=4\delta(t-2\pi),\\
y_0=y(0)=0\\
y_1=y'(0)=0
\end{cases}
$$
Solution:
$$
y(t)=\begin{cases}
0, &0\le t <2\pi \\
4sin(t), & t\ge2\pi
\end{cases}
$$

#####Example5.2 [Zill, p.293]
$$
\begin{cases}
y''+y=4\delta(t-2\pi),\\
y_0=y(0)=1\\
y_1=y'(0)=0
\end{cases}
$$
Solution:
$$
y(t)=cos(t)+4H(t,2\pi)sin(t)
$$
#####Example6
?source
$$
\begin{cases}
x''+9x=3\delta(t-\pi),\\
x_0=x(0)=1\\
x_1=x'(0)=0
\end{cases}
$$
Solution:
$$
x(t)=cos(3t)+H(t,\pi)(-sin(3t))
$$
#####Example7
?source
$$
{\begin{cases}
y''+3y'+2y=\delta(t-1),\\
y_0=y'(0)=0
\end{cases}}
\Rightarrow
{\begin{cases}
y''+3y'+2y=0,\\
y_0=y(1)=0\\
y_1=y'(1_{+})=1
\end{cases}}
$$
#####Example8
?source
$$
\begin{cases}
y''+4y+5y=\delta(t-1),\\
y_0=y(0)=0\\
y_1=y'(0)=3
\end{cases}
$$
Solution:
$$
y(t)=e^{2-2t}H(t,1)sin(t-1)+e^{-2t}sin(t)
$$
#####Example9
?source
$$
\begin{cases}
y''+2y+26y=\delta(t-4),\\
y_0=y(0)=1\\
y_1=y'(0)=0
\end{cases}
$$
Solution:
$$
y(t)=e^{-t}cos(5t)+\frac{1}{5}e^{-t}sin(5t)+\frac{1}{5}H(t,4)e^{-(t-4)}sin(5(t-4))
$$
#####Example10
?source
$$
\begin{cases}
y''+6y'+5y=\delta(t)+\delta(t-2),\\
y_0=y(0)=1\\
y_1=y'(0)=0
\end{cases}
$$
Solution:
$$
y(t)=\frac{3}{2}e^{-t}-\frac{1}{2}e^{-5t}+\frac{1}{4}H(t,2)\left[e^{-t+2}-e^{-5t+10}\right]
$$
#####Example11 [Nagy p.189]
$$
\begin{cases}
y''+2y'+2y=\delta(t),\\
y(0)=y'(0)=0
\end{cases}
$$
Solution:
$$
y(t)=e^{-t}sin(t)
$$
#####Example12 [Nagy p.189]
$$
\begin{cases}
y''+2y'+2y=\delta(t-a),\\
y(0)=y'(0)=0
\end{cases}
$$
Solution:
$$
y(t)=H(t-a)e^{-(t-a)}sin(t-a)
$$
#####Example13 [Nagy p.190]
$$\begin{cases}
y''+4y=\delta(t-\pi)-\delta(t-2\pi),\\
y(0)=y'(0)=0
\end{cases}$$
Solution:
$$y(t)=\frac{1}{2}\left[H(t-\pi)-H(t-2\pi)\right]$$

#####Example14 [Nagy p.189]
$$
\begin{cases}
y''+2y'+2y=\delta(t-a),\\
y(0)=y'(0)=0
\end{cases}
$$
Solution:
$$
y(t)=H(t-a)e^{-(t-a)}sin(t-a)
$$

#####Example15 [Nagy p.190]
$$\begin{cases}
Ty'+y=\delta(t),\\
y(0)=0
\end{cases}$$
Solution:
$$y(t)=\frac{1}{T}e^{-t/T}$$